src/proof/hashtriemap/aux.v
@@ -1,0 +1,42 @@
+(* Things that should be in perennial but arent supported yet *)
+
+From New.generatedproof.hashtriemap Require Import hashtriemap.
+From New.proof Require Import sync.
+From New.proof.sync Require Import atomic.
+From New.proof.sync_proof Require Import mutex.
+From Perennial.algebra Require Import auth_map.
+From Perennial.algebra Require Import ghost_var.
+From Perennial.Helpers Require Import NamedProps.
+Export named_props_ascii_notation.
+From Perennial.Helpers.Word Require Import Integers.
+From coqutil.Word Require Import Interface.
+From iris.algebra Require Import gmap.
+From iris.base_logic.lib Require Import invariants.
+From stdpp Require Import gmap list fin_maps.
+From Coq Require Import List.
+Import ListNotations.
+Open Scope Z_scope.
+
+From Perennial.goose_lang.lib Require Export atomic.impl.
+
+Section aux.
+  Context `{hG: heapGS Σ, !invGS Σ, !ffi_semantics _ _}
+    `{!globalsGS Σ} {go_ctx: GoContext}.
+
+  Parameter atomic_value_model : atomic.Value.t → option loc → Prop.
+  Parameter own_Value : loc -> dfrac -> option val -> iProp Σ.
+
+  (* Using in place of perennial's, since perennial doesnt have std library proofs for atomic Values yet *)
+  Lemma wp_Value__Store (u: loc) (v: val) (Φ : val → iProp Σ) :
+    is_pkg_init atomic -∗
+                          (|={⊤,∅}=> ▷ ∃ old : option val,
+                                         own_Value u (DfracOwn 1) old ∗
+                                           (own_Value u (DfracOwn 1) (Some v) ={∅,⊤}=∗ Φ (# ())))
+    -∗ WP # (method_callv (ptrT.id atomic.Value.id) "Store" (# u)) (v)
+       {{ vret, Φ vret }}.
+  Proof. Admitted.
+
+  #[global] Instance LoadUint32_Atomic (l:loc) : Atomic StronglyAtomic (atomic.LoadUint32 #l).
+  Proof. apply _. Qed.
+  
+End aux.
